---
title: 'Assignment #4'
author: "Elliot Smith"
date: "9/17/2018"
output: pdf_document
---

# Problem 1

# Problem 2

# Problem 3

Solving for $a$ in equation (b) yields:

\[
\begin{aligned}
La & = \ell_\theta \\
a & = \frac{\ell_\theta}{L}
\end{aligned}
\]

Plugging in our result for $a$ into equation (c) yields:

\[
\begin{aligned}
L^T{\theta^*} & = a + e \\
& = \frac{\ell_\theta}{L} + e \\
LL^T{}\theta^* & = \ell_\theta + Le \\
Q_\theta{\theta^*} & = \ell_\theta + Le \\
\theta^* & = \frac{\ell_\theta + Le}{Q_\theta} \\
& = {Q_\theta^{-1}}(\ell_\theta + Le) \\
& = {Q_\theta^{-1}}\ell_\theta + {Q_\theta^{-1}}Le \\
& = {Q_\theta^{-1}}\ell_\theta + N\big[0, (Q_\theta^{-1}L)^TI_d(Q_\theta^{-1}L)\big] \\
& = {Q_\theta^{-1}}\ell_\theta + N\big[0, L^T{Q_\theta^{-1}}^T{Q_\theta^{-1}}L\big] \\
& = {Q_\theta^{-1}}\ell_\theta + N\big[0, \frac{1}{Q_\theta}\big] \\
& = {Q_\theta^{-1}}\ell_\theta + N\big[0, Q_\theta^{-1}\big] \\
& \sim N({Q_\theta^{-1}}\ell_\theta, Q_\theta^{-1})
\end{aligned}
\]

Thus we see that $\theta^* \sim N({Q_\theta^{-1}}\ell_\theta, Q_\theta^{-1})$.