---
title: 'Assignment #3'
author: "Elliot Smith"
date: "9/9/2018"
output: pdf_document
---

# Problem 1

Sampling Distribution: $y_1, ..., y_n|\theta \overset{\text{iid}}{\sim} N(\theta, \sigma^2_y)$
\newline
Prior Distribution: $\theta \sim N(\mu_\theta, \sigma^2_\theta)$
\newline
Posterior Distribution: $\theta|y \sim N(Q^{-1}_\theta{\ell_\theta}, Q^{-1}_\theta)$
\newline
\newline
Posterior Distribution:
\newline
\[
\begin{aligned}
p(\theta|y) & \propto p(y|\theta)p(\theta) \\
& = \Bigg[\frac{1}{\sqrt{2\pi\sigma^2_y}}\Bigg]^n{exp\Bigg(-\frac{1}{2\sigma^2_y}\sum_{i=1}^n(y_i - \theta)^2\Bigg)}
\times \frac{1}{\sqrt{2\pi\sigma^2_\theta}}{exp\Bigg(-\frac{1}{2\sigma^2_\theta}(\theta - \mu_\theta)^2\Bigg)} \\
& \propto {exp\Bigg(-\frac{1}{2\sigma^2_\theta}(\theta - \mu_\theta)^2\Bigg)}
\times {exp\Bigg(-\frac{1}{2\sigma^2_y}\sum_{i=1}^n(y_i - \theta)^2\Bigg)} \\
& = exp\Bigg(-\frac{\theta^2 - 2\theta{\mu_\theta} + \mu_\theta^2}{2\sigma^2_\theta}\Bigg)
\times exp\Bigg(-\frac{\sum_{i=1}^n (y_i^2 - 2\theta{y_i} + \theta^2)}{2\sigma^2_y}\Bigg) \\
& = exp\Bigg(\frac{-\theta^2 + 2\theta{\mu_\theta} - \mu_\theta^2}{2\sigma^2_\theta}
- \frac{\sum_{i=1}^n (y_i^2 - 2\theta{y_i} + \theta^2)}{2\sigma^2_y}\Bigg) \\
& = exp\Bigg(\frac{\sigma^2_y[-\theta^2 + 2\theta{\mu_\theta} - \mu_\theta^2] - \sigma^2_\theta[\sum_{i=1}^n (y_i^2 - 2\theta{y_i} + \theta^2)]}
{2\sigma^2_\theta{\sigma^2_y}}\Bigg) \\
& = exp\Bigg(\frac{-\theta^2(\sigma^2_y + n \sigma^2_\theta) + 2\theta(\mu_\theta\sigma^2_y + \sigma^2_\theta{y_1} + ... + \sigma^2_\theta{y_n})
- (\mu_\theta^2{\sigma^2_y + \sigma^2_\theta{y_1^2}} + ... + \sigma^2_\theta{y_n^2})}{2\sigma^2_\theta{\sigma^2_y}}\Bigg) \\
& = exp\Bigg(\frac{-\theta^2 + 2\theta\frac{\mu_\theta{\sigma^2_y} + \sum_{i=1}^n \sigma^2_\theta{y_i}}{\sigma^2_y + n\sigma^2_\theta} - 
\bigg(\frac{\mu_\theta\sigma^2_y + \sum_{i=1}^n \sigma^2_\theta{y_i}}{\sigma^2_y + n\sigma^2_\theta}\bigg)}{2\frac{\sigma^2_\theta{\sigma^2_y}}{\sigma^2_y + n\sigma^2_\theta}}\Bigg)
\times exp\Bigg(-\frac{\mu_\theta^2\sigma_y^2 + \sum_{i=1}^n \sigma^2_\theta{y_i^2}}{2\sigma^2_\theta\sigma^2_y}\Bigg) \\
& = exp\Bigg(-\frac{\bigg(\theta - \frac{\mu_\theta\sigma^2_y + \sum_{i=1}^n \sigma^2_\theta{y_i}}{\sigma^2_y + n\sigma^2_\theta}\bigg)^2}
{2\frac{\sigma^2_\theta\sigma^2_y}{\sigma^2_y + n\sigma^2_\theta}}\Bigg) \\
\end{aligned}
\]

\newpage

From this result, we can see the following result:
\newline
\[
\begin{aligned}
\theta|y & \sim N\bigg(\frac{\mu_\theta\sigma^2_y + \sum_{i=1}^n \sigma_\theta^2{y_i}}{\sigma^2_y + n\sigma^2_\theta},
\frac{\sigma^2_y\sigma^2_\theta}{\sigma^2_y + n\sigma^2_\theta}\bigg) \\
& \sim N\bigg(\frac{\mu_\theta\sigma^{-2}_\theta + {\sigma_y^{-2}}\sum_{i=1}^n {y_i}}{\sigma^{-2}_\theta + n\sigma^{-2}_y},
\frac{1}{\sigma^{-2}_\theta + n\sigma^{-2}_y}\bigg) \\
& \sim N(Q^{-1}_\theta{\ell_\theta}, Q^{-1}_\theta)
\end{aligned}
\]
\newline
Where the following holds:
\newline
\newline
$Q_\theta = n\sigma^{-2}_y + \sigma^{-2}_\theta$
\newline
$\ell_\theta = \sigma^{-2}_y \sum_{i=1}^n y_i + \sigma^{-2}_\theta{\mu_\theta}$

# Problem 2

## Part i

Posterior Distribution:
\newline
\[
\begin{aligned}
p(\theta|y, \tau_y) & = \frac{1}{\sqrt{2\pi{\sigma^2_y}}}exp\bigg[-\frac{1}{2\sigma^2_y}\sum_{i=1}^n (y_i - \theta{x_i})^2\bigg] \\
& \propto exp\bigg[-\frac{1}{2\sigma^2_y}\sum_{i=1}^n (y_i - \theta{x_i})^2\bigg] \\
& = exp\Bigg[-\frac{1}{2}\bigg(\frac{1}{\sigma^2_y}\sum_{i=1}^n (y_i^2 -2\theta{x_i}{y_i} + \theta^2{x_i^2}\bigg)\Bigg] \\
& = exp\Bigg[-\frac{1}{2}\bigg(\frac{1}{\sigma^2_y}\bigg[\sum_{i=1}^n y_i^2 - \sum_{n=1}^n 2\theta{x_i}{y_i} + \sum_{i=1}^n \theta^2{x_i^2}\bigg]\bigg)\Bigg] \\
& = exp\Bigg[-\frac{1}{2}\bigg(\frac{1}{\sigma^2_y}\bigg[\sum_{i=1}^n y_i^2 - {2\theta}\sum_{n=1}^n {x_i}{y_i} + {\theta^2} \sum_{i=1}^n {x_i^2}\bigg]\bigg)\Bigg] \\
& = exp\Bigg[-\frac{1}{2}\bigg(\sigma^{-2}_y\sum_{i=1}^n y_i^2 - {2\theta}\sigma^{-2}_y\sum_{n=1}^n {x_i}{y_i} + {\theta^2}\sigma^{-2}_y \sum_{i=1}^n {x_i^2}\bigg)\Bigg] \\
& \propto exp\Bigg[-\frac{1}{2}\bigg({\theta^2}\sigma^{-2}_y \sum_{i=1}^n {x_i^2} - {2\theta}\sigma^{-2}_y\sum_{n=1}^n {x_i}{y_i}\bigg)\Bigg] \\
\end{aligned}
\]
\newline
Now, given the formula: $p(\theta|y) \propto exp\bigg[-\frac{1}{2}\bigg(Q_\theta{\theta^2} - 2\ell_\theta{\theta}\bigg)\bigg]$
\newline
\newline
We get the results that:
\newline
\newline
$Q_\theta = \sigma^{-2}_y \sum_{i=1}^n {x_i^2}$
\newline
$\ell_\theta = \sigma^{-2}_y\sum_{n=1}^n {x_i}{y_i}$
\newline
\[
\begin{aligned}
p(\theta|y, \tau_y) & \sim N(Q_\theta^{-1}\ell_\theta, Q_\theta^{-1}) \\
& \sim N\bigg(\big(\sigma^{-2}_y \sum_{i=1}^n {x_i^2}\big)^{-1} \times \big(\sigma^{-2}_y\sum_{n=1}^n {x_i}{y_i}\big)^{-1}, \big(\sigma^{-2}_y \sum_{i=1}^n {x_i^2}\big)^{-1} \bigg)
\end{aligned}
\]

# Problem 3

Sampling Distribution: $p(y|\theta) = \frac{\theta^ye^-\theta}{y!}$
\newline
Domain: $\theta > 0$
\newline
\newline
\[
\begin{aligned}
p(y|\theta) & = \prod_{i=1}^{n}\frac{\theta^{y_i}e^-{\theta}}{{y_i}!} \\
& = \theta^{{\sum_{i=1}^n}{y_i}}e^{-n\theta} \times \prod_{i=1}^n \frac{1}{{y_i}!} \\
log[p(y|\theta)] & = log\bigg[\theta^{{\sum_{i=1}^n}{y_i}}e^{-n\theta} \times \prod_{i=1}^n \frac{1}{{y_i}!}\bigg] \\
& = \bigg[{\sum_{i=1}^n}{y_i}\bigg]log(\theta) - n\theta - log\bigg[\sum_{i=1}^n{y_i}!\bigg] \\
\frac{d}{d\theta}log[p(y|\theta)] & = \frac{d}{d\theta}\Bigg[\bigg[{\sum_{i=1}^n}{y_i}\bigg]log(\theta)\Bigg]  - \frac{d}{d\theta}({n\theta}) + 0\\
& = \bigg[\sum_{i=1}^n{y_i}\bigg]{\frac{1}{\theta}} - n \\
\frac{d^2}{d\theta^2}log[p(y|\theta)] & = \bigg[\sum_{i=1}^n\frac{d}{d\theta} \theta^{-1}\bigg] + 0 \\
& = \frac{-\sum_{i=1}^n{y_i}}{\theta^2} \\
E\bigg[\frac{d^2log[p(y|\theta)]}{d\theta^2}\bigg|\theta\bigg] & = \frac{-n\theta}{\theta^2} \\
& = \frac{-n}{\theta} \\
\sqrt{-E\bigg[\frac{d^2log[p(y|\theta)]}{d\theta^2}\bigg|\theta\bigg]} & = \sqrt{\frac{n}{\theta}} \\
& \propto \theta^{-\frac{1}{2}} \\
& \sim Gamma\bigg(\alpha = \frac{1}{2}, \beta = 0\bigg)
\end{aligned}
\]










